theories/algebra/base_extra.v
@@ -1,4 +1,5 @@
 From HypVeri.algebra Require Import base.
+From HypVeri Require Import stdpp_extra.
 
 Section predicates.
 
@@ -97,9 +98,16 @@ Section preservation.
     rewrite /inv_trans_pgt_consistent Heq_proj_trans Heq_proj_pgt //.
   Qed.
 
+  Lemma preserve_inv_trans_ps_disj σ' σ :
+    (get_transactions σ) = (get_transactions σ') -> inv_trans_ps_disj σ = inv_trans_ps_disj σ'.
+  Proof.
+    intro Heq_proj.
+    rewrite /inv_trans_ps_disj Heq_proj //.
+  Qed.
+
 End preservation.
 
-Section helper.
+Section helpers.
 
   Context `{hypconst : !HypervisorConstants}.
 
@@ -113,8 +121,463 @@ Section helper.
                                 end
                     ).
 
-End helper.
+  (* lemmas about pages_in_trans *)
+  Lemma elem_of_pages_in_trans' p trans:
+    p ∈ pages_in_trans' trans <-> ∃ h tran, trans !! h = Some (Some tran) ∧ p ∈ tran.1.1.2.
+  Proof.
+    rewrite /pages_in_trans'.
+    induction trans using map_ind.
+    {
+      rewrite map_fold_empty //.
+      split;intros;first done.
+      destruct H as [? [? [? ?]]].
+      done.
+    }
+    {
+      rewrite map_fold_insert_L.
+      2:{
+        intros w1 w2 trans1 trans2 y.
+        intros Hneq Hlookup1 Hlookup2.
+        destruct trans1, trans2;
+        set_solver +.
+      }
+      2: done.
+      destruct x as [x|].
+      + rewrite elem_of_union.
+        split;intro Hin.
+        destruct Hin as [Hin|Hin].
+        exists i, x.
+        split;auto.
+        rewrite lookup_insert_Some;left;done.
+        apply IHtrans in Hin as [h [x' [Hlookup Hin']]].
+        exists h, x'.
+        split;auto.
+        rewrite lookup_insert_Some;right.
+        split;auto.
+        intro.
+        subst i.
+        rewrite H // in Hlookup.
+        destruct (decide (p ∈ x.1.1.2)).
+        left;done.
+        right.
+        apply IHtrans.
+        destruct Hin as [h [x' [Hlookup Hin']]].
+        destruct (decide (i = h)).
+        subst i.
+        rewrite lookup_insert_Some in Hlookup.
+        destruct Hlookup as [? | [? ?]].
+        destruct H0;subst.
+        inversion H1;subst.
+        contradiction.
+        contradiction.
+        exists h, x'.
+        split;last done.
+        rewrite lookup_insert_ne in Hlookup.
+        done.
+        done.
+      + rewrite IHtrans.
+        split.
+        intros [h [tran [Hlookup Hin]]].
+        exists h, tran.
+        split;auto.
+        destruct (decide (i= h)).
+        subst i. rewrite H in Hlookup; done.
+        rewrite lookup_insert_ne //.
+        intros [h [tran [Hlookup Hin]]].
+        destruct (decide (i= h)).
+        subst i. rewrite lookup_insert_Some in Hlookup.
+        destruct Hlookup as [[_ ?]|[? _]];done.
+        exists h, tran.
+        split;auto.
+        rewrite lookup_insert_ne in Hlookup;auto.
+    }
+  Qed.
 
+  Lemma subseteq_pages_in_trans' h tran trans:
+    trans !! h = Some (Some tran) ->
+    tran.1.1.2 ⊆ pages_in_trans' trans.
+  Proof.
+    intros Hlk.
+    rewrite /pages_in_trans'.
+    induction trans using map_ind.
+    {
+      rewrite map_fold_empty //.
+    }
+    {
+      rewrite map_fold_insert_L.
+      2:{
+        intros w1 w2 trans1 trans2 y.
+        intros Hneq Hlookup1 Hlookup2.
+        destruct trans1, trans2;
+        set_solver +.
+      }
+      2: done.
+      destruct (decide (i = h)).
+      {
+        subst i.
+        rewrite lookup_insert in Hlk.
+        inversion Hlk.
+        subst x.
+        set_solver +.
+      }
+      {
+        feed specialize IHtrans.
+        rewrite lookup_insert_ne in Hlk;auto.
+        destruct x;
+        set_solver + IHtrans.
+      }
+    }
+  Qed.
+
+  Lemma pages_in_trans_subseteq' m m':
+    m' ⊆ m -> pages_in_trans' m' ⊆ pages_in_trans' m.
+  Proof.
+    intros Hsub.
+    rewrite /pages_in_trans'.
+    induction m' using map_ind.
+    {
+      rewrite map_fold_empty //.
+    }
+    {
+      rewrite map_fold_insert_L.
+      2:{
+        intros w1 w2 trans1 trans2 y.
+        intros Hneq Hlookup1 Hlookup2.
+        destruct trans1, trans2;
+        set_solver +.
+      }
+      2: done.
+      pose proof Hsub.
+      rewrite map_subseteq_spec in Hsub.
+      specialize (Hsub i x).
+      feed specialize Hsub.
+      rewrite lookup_insert //.
+      destruct x as [x|].
+      + apply union_least.
+        {
+          rewrite elem_of_subseteq.
+          intros.
+          rewrite elem_of_pages_in_trans'.
+          exists i, x.
+          split;done.
+        }
+        apply IHm'.
+        rewrite map_subseteq_spec.
+        intros.
+        rewrite map_subseteq_spec in H0.
+        apply H0.
+        rewrite lookup_insert_Some.
+        right.
+        split;last done.
+        intro.
+        subst.
+        rewrite H1 in H.
+        done.
+      + apply IHm'.
+        apply map_subseteq_spec.
+        intros.
+        rewrite map_subseteq_spec in H0.
+        apply (H0 i0 x).
+        destruct (decide (i = i0)).
+        subst i0.
+        rewrite H // in H1.
+        rewrite lookup_insert_ne //.
+    }
+  Qed.
+
+  Lemma pages_in_trans_insert_None'{h tran trans}:
+    trans !! h = None ->
+    pages_in_trans' (<[h := Some tran]> trans) = tran.1.1.2 ∪ pages_in_trans' trans.
+  Proof.
+    intros Hlk.
+    rewrite /pages_in_trans'.
+    rewrite map_fold_insert_L.
+    2:{
+      intros w1 w2 trans1 trans2 y.
+      intros Hneq Hlookup1 Hlookup2.
+      destruct trans1, trans2;
+      set_solver +.
+    }
+    2: done.
+    done.
+  Qed.
+
+  Lemma pages_in_trans_insert_Some'{h tran tran' trans}:
+    trans !! h = Some (Some tran) ->
+    tran.1 = tran'.1 ->
+    pages_in_trans' (<[h := Some tran']> trans) = pages_in_trans' trans.
+  Proof.
+    intros Hlk.
+    rewrite /pages_in_trans'.
+    induction trans using map_ind.
+    {
+      rewrite map_fold_empty //.
+    }
+    {
+      intro Heq.
+      destruct (decide (i = h)).
+      subst i.
+      rewrite insert_insert.
+      rewrite lookup_insert_Some in Hlk.
+      destruct Hlk as [[_ ->]|[? _]].
+      2: done.
+      rewrite map_fold_insert_L;auto.
+      2:{
+        intros w1 w2 trans1 trans2 y.
+        intros Hneq Hlookup1 Hlookup2.
+        destruct trans1, trans2;
+        set_solver +.
+      }
+      rewrite map_fold_insert_L;auto.
+      2:{
+        intros w1 w2 trans1 trans2 y.
+        intros Hneq Hlookup1 Hlookup2.
+        destruct trans1, trans2;
+        set_solver +.
+      }
+      rewrite Heq //.
+      rewrite lookup_insert_Some in Hlk.
+      destruct Hlk as [[? _]|[_ Hlk]].
+      contradiction.
+      rewrite map_insert_swap //.
+      specialize (IHtrans Hlk Heq).
+      rewrite (map_fold_insert_L _ _ _ _ (<[h:=tran']> m));auto.
+      2:{
+        intros w1 w2 trans1 trans2 y.
+        intros Hneq Hlookup1 Hlookup2.
+        destruct trans1, trans2;
+        set_solver +.
+      }
+      rewrite (map_fold_insert_L _ _ i _ );auto.
+      2:{
+        intros w1 w2 trans1 trans2 y.
+        intros Hneq Hlookup1 Hlookup2.
+        destruct trans1, trans2;
+        set_solver +.
+      }
+      2: rewrite lookup_insert_ne //.
+      rewrite IHtrans //.
+    }
+Qed.
+
+  Lemma trans_ps_disj_subseteq' m m':
+    inv_trans_ps_disj' m -> m' ⊆ m -> inv_trans_ps_disj' m'.
+  Proof.
+    intros Hdisj Hsub.
+    intros k v Hlookup.
+    rewrite map_subseteq_spec in Hsub.
+    assert (delete k m' ⊆ delete k m).
+    rewrite map_subseteq_spec.
+    intros.
+    destruct (decide (i = k)).
+    {
+      subst.
+      rewrite lookup_delete_Some in H.
+      destruct H;contradiction.
+    }
+    {
+      rewrite lookup_delete_ne in H;auto.
+      rewrite lookup_delete_ne;auto.
+    }
+    pose proof (pages_in_trans_subseteq' _ _ H).
+    specialize (Hdisj k v).
+    simpl in Hdisj.
+    feed specialize Hdisj.
+    apply Hsub;eauto.
+    destruct v;auto.
+    set_solver + Hdisj H0.
+  Qed.
+
+  Lemma pages_in_trans_delete' {h tran trans}:
+    trans !! h = Some (Some tran) ->
+    inv_trans_ps_disj' trans ->
+    pages_in_trans' (delete h trans) = pages_in_trans' trans ∖ tran.1.1.2.
+  Proof.
+    intros Hlk Hdisj.
+    specialize (Hdisj _ _ Hlk).
+    rewrite /pages_in_trans'.
+    induction trans using map_ind.
+    {
+      rewrite map_fold_empty //.
+    }
+    {
+      rewrite map_fold_insert_L.
+      2:{
+        intros w1 w2 trans1 trans2 y.
+        intros Hneq Hlookup1 Hlookup2.
+        destruct trans1, trans2;
+        set_solver +.
+      }
+      2: done.
+      destruct (decide (i = h)).
+      subst i.
+      rewrite delete_insert. 2: done.
+      {
+        simpl in Hdisj.
+        rewrite lookup_insert in Hlk.
+        inversion Hlk.
+        subst x.
+        clear Hlk.
+        rewrite delete_insert in Hdisj;auto.
+        rewrite /pages_in_trans' in Hdisj.
+        set_solver + Hdisj.
+      }
+      {
+        rewrite delete_insert_ne;auto.
+        rewrite map_fold_insert_L.
+        2:{
+          intros w1 w2 trans1 trans2 y.
+          intros Hneq Hlookup1 Hlookup2.
+          destruct trans1, trans2;
+          set_solver +.
+        }
+        2: {
+          rewrite lookup_delete_ne;auto.
+        }
+        rewrite lookup_insert_ne in Hlk.
+        rewrite delete_insert_ne in Hdisj;auto.
+        rewrite /pages_in_trans' in Hdisj.
+        rewrite map_fold_insert_L in Hdisj.
+        2:{
+          intros w1 w2 trans1 trans2 y.
+          intros Hneq Hlookup1 Hlookup2.
+          destruct trans1, trans2;
+          set_solver +.
+        }
+        2: {
+          rewrite lookup_delete_ne;auto.
+        }
+        rewrite /pages_in_trans'.
+        destruct x.
+        rewrite IHtrans;auto.
+        2: set_solver + Hdisj.
+        set_solver + Hdisj.
+        2: done.
+        rewrite IHtrans;auto.
+      }
+    }
+  Qed.
+
+  Lemma trans_ps_disj_insert' h tran trans :
+    inv_trans_ps_disj' trans ->
+    trans !! h = None ->
+    tran.1.1.2 ## pages_in_trans' trans ->
+    inv_trans_ps_disj' (<[h:=Some tran]> trans).
+  Proof.
+    intros Hdisj Hlk Hdisj'.
+    intros k v Hlk'.
+    destruct (decide (k = h)).
+    {
+      subst.
+      rewrite delete_insert;auto.
+      rewrite lookup_insert in Hlk'.
+      inversion Hlk'.
+      subst v.
+      done.
+    }
+    {
+      rewrite delete_insert_ne;auto.
+      destruct v as [v|];auto.
+      rewrite lookup_insert_ne in Hlk';auto.
+      rewrite (pages_in_trans_insert_None').
+      rewrite (pages_in_trans_delete' Hlk' );auto.
+      pose proof (subseteq_pages_in_trans' _ _ _ Hlk').
+      set_solver + Hdisj' H.
+      rewrite lookup_delete_ne;auto.
+    }
+  Qed.
+
+  Lemma trans_ps_disj_update'{trans h tran tran'}:
+    inv_trans_ps_disj' trans ->
+    trans !! h = Some (Some tran)->
+    tran.1 = tran'.1 ->
+    inv_trans_ps_disj' (<[h:= Some tran']> trans).
+  Proof.
+    intros Hdisj Hlk Heq.
+    intros k v Hlk'.
+    destruct (decide (k = h)).
+    {
+      subst.
+      rewrite delete_insert_delete;auto.
+      rewrite lookup_insert in Hlk'.
+      inversion Hlk'.
+      subst v.
+      rewrite -Heq.
+      specialize (Hdisj h (Some tran) Hlk).
+      simpl in Hdisj.
+      done.
+    }
+    {
+      rewrite delete_insert_ne;auto.
+      rewrite (pages_in_trans_insert_Some' (tran:=tran));auto.
+      rewrite lookup_insert_ne in Hlk';auto.
+      destruct v as [v|];auto.
+      specialize (Hdisj k (Some v) Hlk').
+      simpl in Hdisj.
+      done.
+      rewrite lookup_delete_ne //.
+    }
+  Qed.
+
+  Lemma trans_ps_disj_delete'{trans h}:
+    inv_trans_ps_disj' trans ->
+    (* trans !! h = Some (Some tran)-> *)
+    inv_trans_ps_disj' (<[h:= None]> trans).
+  Proof.
+    intros Hdisj.
+    intros k v Hlk'.
+    destruct (decide (k = h)).
+    {
+      subst.
+      rewrite delete_insert_delete;auto.
+      rewrite lookup_insert in Hlk'.
+      inversion Hlk'.
+      subst v.
+      done.
+    }
+    {
+      rewrite delete_insert_ne;auto.
+      rewrite lookup_insert_ne in Hlk';auto.
+      destruct v as [v|];auto.
+      specialize (Hdisj k (Some v) Hlk').
+      simpl in Hdisj.
+      rewrite -insert_delete_insert.
+      rewrite /pages_in_trans'.
+      rewrite map_fold_insert_L.
+      assert (delete h (delete k trans) ⊆ delete k trans).
+      { apply map_subseteq_delete. }
+      apply pages_in_trans_subseteq' in H.
+      set_solver + H Hdisj.
+      {
+        intros.
+        destruct z1,z2;set_solver.
+      }
+      rewrite lookup_delete_None.
+      eauto.
+    }
+  Qed.
+
+(* we don't have actual deletion *)
+  (* Lemma trans_ps_disj_delete' {trans h tran}: *)
+  (*   trans !! h = Some tran -> *)
+  (*   inv_trans_ps_disj' trans -> *)
+  (*   inv_trans_ps_disj' (delete h trans). *)
+  (* Proof. *)
+  (*   rewrite /inv_trans_ps_disj'. *)
+  (*   intros Hlk Hdisj. *)
+  (*   pose proof Hdisj as Hdisj'. *)
+  (*   apply map_Forall_delete. *)
+  (*   intros h' tran' Hlk'. *)
+  (*   specialize (Hdisj h' tran' Hlk'). *)
+  (*   simpl in Hdisj. *)
+  (*   destruct tran';auto. *)
+  (*   assert (delete h' (delete h trans) ⊆ delete h' trans). *)
+  (*   { rewrite delete_commute. apply map_subseteq_delete. } *)
+  (*   apply pages_in_trans_subseteq' in H. *)
+  (*   set_solver + H Hdisj. *)
+  (* Qed. *)
+
+End helpers.
 
 From iris.algebra.lib Require Import gmap_view.
 
@@ -140,4 +603,4 @@ Section ghost_map_extra.
     done.
   Qed.
 
-  End ghost_map_extra.
+End ghost_map_extra.
