theories/logrel/fundamental.v
@@ -2,7 +2,7 @@ From iris.proofmode Require Import tactics.
 From machine_program_logic.program_logic Require Import weakestpre.
 From HypVeri.lang Require Import lang trans_extra.
 From HypVeri.algebra Require Import base pagetable mem trans.
-From HypVeri.rules Require Import rules_base nop mov yield ldr halt fail add sub mult cmp br bne str run.
+From HypVeri.rules Require Import rules_base mov yield ldr halt fail add sub mult cmp br bne str run.
 From HypVeri.logrel Require Import logrel logrel_extra.
 From HypVeri.logrel Require Import ftlr_nop ftlr_run ftlr_yield ftlr_share ftlr_retrieve ftlr_msg_send
      ftlr_msg_wait ftlr_msg_poll ftlr_relinquish ftlr_reclaim ftlr_donate ftlr_lend ftlr_invalid_hvc.
