theories/rules/bne.v
@@ -80,8 +80,9 @@ Proof.
       rewrite (preserve_get_retri_gmap σ1).
       rewrite (preserve_inv_trans_pgt_consistent σ1).
       rewrite (preserve_inv_trans_wellformed σ1).
+      rewrite (preserve_inv_trans_ps_disj σ1).
       rewrite p_upd_pc_mem.
-      all: try rewrite p_upd_pc_trans //.    
+      all: try rewrite p_upd_pc_trans //.
       all: try rewrite p_upd_pc_pgt //.    
       all: try rewrite p_upd_pc_mb //.
       iFrame.
@@ -137,6 +138,7 @@ Proof.
       rewrite (preserve_get_retri_gmap σ1).
       rewrite (preserve_inv_trans_pgt_consistent σ1).
       rewrite (preserve_inv_trans_wellformed σ1).
+      rewrite (preserve_inv_trans_ps_disj σ1).
       all: try rewrite p_upd_reg_pgt //.
       all: try rewrite p_upd_reg_trans //.
       all: try rewrite p_upd_reg_mb //.
