theories/rules/cmp.v
@@ -65,6 +65,7 @@ Proof.
     rewrite (preserve_get_retri_gmap σ1).
     rewrite (preserve_inv_trans_pgt_consistent σ1).
     rewrite (preserve_inv_trans_wellformed σ1).
+    rewrite (preserve_inv_trans_ps_disj σ1).
     rewrite p_upd_pc_mem p_upd_reg_mem.
     all: try rewrite p_upd_pc_pgt p_upd_reg_pgt //.
     all: try rewrite p_upd_pc_trans p_upd_reg_trans //.
@@ -298,6 +299,7 @@ Proof.
     rewrite (preserve_get_retri_gmap σ1).
     rewrite (preserve_inv_trans_pgt_consistent σ1).
     rewrite (preserve_inv_trans_wellformed σ1).
+    rewrite (preserve_inv_trans_ps_disj σ1).
     rewrite p_upd_pc_mem p_upd_reg_mem.
     all: try rewrite p_upd_pc_pgt p_upd_reg_pgt //.
     all: try rewrite p_upd_pc_trans p_upd_reg_trans //.
