theories/rules/nop.v
@@ -66,6 +66,7 @@ Proof.
     rewrite (preserve_get_retri_gmap σ1).
     rewrite (preserve_inv_trans_pgt_consistent σ1).
     rewrite (preserve_inv_trans_wellformed σ1).
+    rewrite (preserve_inv_trans_ps_disj σ1).
     rewrite p_upd_pc_mem.
     all: try rewrite p_upd_pc_pgt //.
     all: try rewrite p_upd_pc_trans //.
