theories/rules/run.v
@@ -92,6 +92,7 @@ Proof.
     rewrite (preserve_get_retri_gmap σ1).
     rewrite (preserve_inv_trans_pgt_consistent σ1).
     rewrite (preserve_inv_trans_wellformed σ1).
+    rewrite (preserve_inv_trans_ps_disj σ1).
     all: try rewrite p_upd_id_mb p_upd_pc_mb //.
     all: try rewrite p_upd_id_pgt p_upd_pc_pgt //.
     all: try rewrite p_upd_id_trans p_upd_pc_trans //.
