theories/rules/yield.v
@@ -94,6 +94,7 @@ Proof.
       rewrite (preserve_get_retri_gmap σ1).
       rewrite (preserve_inv_trans_pgt_consistent σ1).
       rewrite (preserve_inv_trans_wellformed σ1).
+      rewrite (preserve_inv_trans_ps_disj σ1).
       all: try rewrite p_upd_id_mb p_upd_pc_mb //.
       all: try rewrite p_upd_id_pgt p_upd_pc_pgt //.
       all: try rewrite p_upd_id_trans p_upd_pc_trans //.
@@ -156,7 +157,6 @@ Proof.
           apply H1.
           apply V0eq.
         }
-
         assert (In 0 (seq 0 vm_count)) as Prf'.
         {
           rewrite <-elem_of_list_In.
